solution for revised ch04/ex02

chapter04/solutions/exercise02_solution.dfy
@@ -1,77 +1,94 @@
-module LockServer {
+datatype ServerGrant = Unlocked | Client(id: nat)
 
-  datatype Option<V> = None | Some(value:V)
-  function NumClients() : int ensures NumClients() > 0
-  newtype ClientId = b: int | 0 <= b < NumClients()
-  type ClientMap = m: map<ClientId, bool> | forall c :: c in m
-    witness map k:ClientId | true :: false
+datatype ClientRecord = Released | Acquired
 
-  datatype Constants = Constants()
-  datatype Variables = Variables(holder:Option<ClientId>, clientHolds:ClientMap)
+datatype State = State(server: ServerGrant, clients: seq<ClientRecord>)
 
-  predicate Init(k:Constants, s:Variables) {
-    && s.holder.None?
-    && forall c :: !s.clientHolds[c]
-  }
+predicate Init(s: State) {
+  && s.server.Unlocked?
+  && forall i | 0 <= i < |s.clients| :: s.clients[i].Released?
+}
 
-  predicate Grant(k:Constants, s:Variables, s':Variables, toClient:ClientId) {
-    && s.holder.None?
-    && s'.holder == Some(toClient)  // Omitted for proof debug trap
-    && s'.clientHolds == s.clientHolds[toClient := true]
-  }
+predicate Acquire(s: State, s':State, id:int) {
+  && 0 <= id < |s.clients|
 
-  predicate Return(k:Constants, s:Variables, s':Variables, fromClient:ClientId) {
-    && s.holder == Some(fromClient)
-    && s'.holder.None?
-    && s'.clientHolds == s.clientHolds[fromClient := false]
-  }
+  // Enabling condition: The server checks its local state.
+  && s.server.Unlocked?
 
-  datatype Step = GrantStep(toClient:ClientId) | ReturnStep(fromClient:ClientId)
+  // Update the server state.
+  && s'.server == Client(id)
 
-  predicate NextStep(k:Constants, s:Variables, s':Variables, step:Step) {
-    match step {
-      case GrantStep(toClient) => Grant(k, s, s', toClient)
-      case ReturnStep(fromClient) => Grant(k, s, s', fromClient)
-    }
-  }
+  // Update the client that acquired.
+  && |s'.clients| == |s.clients|  // Don't lose track of any clients.
+  && ( forall i | 0 <= i < |s.clients| ::
+      s'.clients[i] == if i == id then Acquired else s.clients[i] )
+}
 
-  predicate Next(k:Constants, s:Variables, s':Variables) {
-    exists step :: NextStep(k, s, s', step)
+predicate Release(s: State, s':State, id:int) {
+  && 0 <= id < |s.clients|
+
+  // Enabling condition: The client trying to release checks its local state.
+  && s.clients[id].Acquired?
+
+  // Update the server state.
+  && s'.server.Unlocked?
+
+  // Update the client that released.
+  && |s'.clients| == |s.clients|  // Don't lose track of any clients.
+  && ( forall i | 0 <= i < |s.clients| ::
+      s'.clients[i] == if i == id then Released else s.clients[i] )
+}
+
+datatype Step = AcquireStep(id:int) | ReleaseStep(id:int)
+
+predicate NextStep(s:State, s':State, step:Step) {
+  match step {
+    case AcquireStep(toClient) => Acquire(s, s', toClient)
+    case ReleaseStep(fromClient) => Release(s, s', fromClient)
   }
 }
 
-module LockServerProof {
-  import opened LockServer
+predicate Next(s:State, s':State) {
+  exists step :: NextStep(s, s', step)
+}
 
-  predicate Safety(k:Constants, s:Variables) {
-    forall c1, c2 :: s.clientHolds[c1] && s.clientHolds[c2] ==> c1 == c2
-  }
-  
-  predicate ServerExcludesClients(k:Constants, s:Variables) {
-    s.holder.None? ==> (forall c :: !s.clientHolds[c])
-  }
+predicate Safety(s:State) {
+  // What's a good definition of safety for the lock server? No two clients
+  // have the lock simultaneously. Write that here.
+  forall i,j ::
+    (&& 0 <= i < |s.clients|
+    && 0 <= j < |s.clients|
+    && s.clients[i].Acquired?
+    && s.clients[j].Acquired?) ==> i == j
+}
 
-  predicate Inv(k:Constants, s:Variables) {
-    && Safety(k, s)
-    && ServerExcludesClients(k, s)
-  }
+// Safety doesn't care what server thinks, but to get an *inductive* invariant,
+// we need to ensure the server doesn't fall out of sync with the clients'
+// beliefs.
+predicate ServerAgreesClients(s:State) {
+  s.server.Unlocked? <==> (forall id | 0 <= id < |s.clients| :: s.clients[id].Released?)
+}
 
-  lemma InvInit(k:Constants, s:Variables, s':Variables)
-    requires Init(k, s)
-    ensures Inv(k, s)
-  {
-  }
+predicate Inv(s:State) {
+  && Safety(s)
+  && ServerAgreesClients(s)
+}
 
-  lemma InvNext(k:Constants, s:Variables, s':Variables)
-    requires Next(k, s, s')
-    requires Inv(k, s)
-    ensures Inv(k, s')
-  {
-  }
-
-  lemma InvImpliesSafety(k:Constants, s:Variables)
-    requires Inv(k, s)
-    ensures Safety(k, s)
-  {
+// Here's your obligation. Probably easiest to break this up into three
+// lemmas, each P==>Q becomes requires P ensures Q.
+lemma SafetyTheorem(s:State, s':State)
+  ensures Init(s) ==> Inv(s)
+  ensures Inv(s) && Next(s, s') ==> Inv(s')
+  ensures Inv(s) ==> Safety(s)
+{
+  if Inv(s) && Next(s, s') {
+    var step :| NextStep(s, s', step);        // give a variable name ("step") to what happened in Next
+    if step.AcquireStep? {                    // case analysis
+//      assert !s'.server.Unlocked?;
+      assert !s'.clients[step.id].Released?;  // witness to exist (!forall in ServerAgreesClient)
+//      assert Inv(s');
+//    } else {
+//      assert Inv(s');
+    }
   }
 }
